Refactor bitvec and add TODOs

lean/bitvec.lean
@@ -11,7 +11,8 @@ import data.vector
 
 import .common -- for dec_trivial_tac
 
-@[reducible] def bitvec (sz:ℕ) :=
+@[reducible]
+def bitvec (sz:ℕ) :=
   { x : ℕ // x < (2 ^ sz) }
 
 namespace bitvec
@@ -19,21 +20,20 @@ open nat
 open vector
 
 -- Create a zero bitvector
-@[reducible] protected
+protected
 def zero (n : ℕ) : bitvec n :=
   ⟨0, nat.pos_pow_of_pos n dec_trivial⟩
 
 instance {n:ℕ} : has_zero (bitvec n) := ⟨bitvec.zero n⟩
 
 -- Create a bitvector with the constant one.
-@[reducible] protected
+protected
 def one_of_pos_len (n: ℕ) {H : n > 0} : bitvec n :=
   ⟨1, calc
-        1   < 2   : by dec_trivial_tac
-        ... = 2^1 : by trivial
+        1   < 2^1 : by dec_trivial_tac
         ... ≤ 2^n : by apply (pow_le_pow_of_le_right (zero_lt_succ _) (succ_le_of_lt H))⟩
 
-@[reducible] protected
+protected
 def one (n:ℕ) : bitvec n :=
   begin
     cases n,
@@ -50,6 +50,7 @@ instance {n:ℕ} : has_one (bitvec n)  := ⟨bitvec.one n⟩
 protected def cong {a b : ℕ} (h : a = b) : bitvec a → bitvec b
 | ⟨x, p⟩ := ⟨x, h ▸ p⟩
 
+@[simp]
 lemma in_range (x n : ℕ) : x % 2 ^ n < 2 ^ n :=
   begin
     apply (mod_lt _),
@@ -57,17 +58,25 @@ lemma in_range (x n : ℕ) : x % 2 ^ n < 2 ^ n :=
     simp [zero_lt_succ]
   end
 
--- bitvec specific version of vector.append
-def append {m n} (x: bitvec m) (y: bitvec n) : bitvec (m + n) := ⟨ (x.val * 2^n + y.val) % 2^(m + n), by simp [in_range] ⟩
+-- TODO: move this lemmas to a nat lemma module, see lean protocol buffers repo for example
 
-lemma div_lt_of_lt_mul {m n : ℕ} : ∀ {k} (Hk : k > 0), m < k * n → m / k < n
-  | 0        Hk h := by apply absurd Hk (lt_irrefl 0)
-  | (succ k) Hk h :=
-    suffices succ k * (m / succ k) < succ k * n, from lt_of_mul_lt_mul_left this (zero_le _),
-    calc
-      succ k * (m / succ k) ≤ m % succ k + succ k * (m / succ k) : le_add_left _ _
-                        ... = m                                  : by rw mod_add_div
-                        ... < succ k * n                         : h
+lemma lt_one_is_zero {x:ℕ} : x < 1 ↔ x = 0 :=
+  begin
+    constructor,
+    { intros,
+      apply eq_zero_of_le_zero (le_of_lt_succ _),
+      assumption },
+    { intros, simp [a], dec_trivial_tac }
+  end
+
+@[simp]
+lemma bitvec_zero_zero (x : bitvec 0) : x.val = 0 :=
+  begin
+    cases x,
+    { simp [nat.pow_zero, lt_one_is_zero] at x_property,
+      simp, assumption
+    }
+  end
 
 lemma pow_mul {b n m :ℕ} : b^n * b^m = b^(n+m) :=
   begin
@@ -77,6 +86,34 @@ lemma pow_mul {b n m :ℕ} : b^n * b^m = b^(n+m) :=
     case nat.succ
     { rw [pow_succ, ←mul_assoc (b^n), m_ih, ←pow_succ] }
   end
+
+lemma mul_pow_add_lt_pow {x y n m:ℕ} (Hx: x < 2^m) (Hy: y < 2^n) : x * 2^n + y < 2^(m + n) :=
+  calc
+    x*2^n + y < x*2^n + 2^n   : nat.add_lt_add_left Hy (x*2^n)
+          ... = (x + 1) * 2^n : begin rw right_distrib, simp end
+          ... ≤ 2^m * 2^n     : nat.mul_le_mul_right (2^n) (succ_le_of_lt Hx)
+          ... = 2^(m + n)     : pow_mul
+
+
+def zext {n:ℕ} (m:ℕ) (x: bitvec n) : bitvec (n+m) :=
+  ⟨ x.val, calc x.val < 2^n     : x.property
+                  ... ≤ 2^(n+m) : begin
+                                    apply pow_le_pow_of_le_right, dec_trivial_tac,
+                                    apply le_add_right
+                                  end⟩
+
+-- bitvec specific version of vector.append
+def append {m n} (x: bitvec m) (y: bitvec n) : bitvec (m + n)
+  := ⟨ x.val * 2^n + y.val, mul_pow_add_lt_pow x.property y.property ⟩
+
+lemma div_lt_of_lt_mul {m n : ℕ} : ∀ {k} (Hk : k > 0), m < k * n → m / k < n
+  | 0        Hk h := by apply absurd Hk (lt_irrefl 0)
+  | (succ k) Hk h :=
+    suffices succ k * (m / succ k) < succ k * n, from lt_of_mul_lt_mul_left this (zero_le _),
+    calc
+      succ k * (m / succ k) ≤ m % succ k + succ k * (m / succ k) : le_add_left _ _
+                        ... = m                                  : by rw mod_add_div
+                        ... < succ k * n                         : h
 
 lemma sub_lt_left {a b} (c:ℕ) (H: a < b) (Ha: a > c) : a - c < b - c :=
   begin
@@ -132,24 +169,113 @@ lemma sub_add_lt_self (a b c : ℕ) (Hab: a > b) (Hbc : b > c) : a - b + c < a :
 section shift
   variable {n : ℕ}
 
-  @[reducible]
-  def shl (x : bitvec n) (i : ℕ) : bitvec n := ⟨x.val * 2^i % 2^n, by simp [in_range]⟩
+  def shl (x : bitvec n) (i : ℕ) : bitvec n := ⟨x.val * 2^i % 2^n, by simp⟩
 
-  @[reducible]
   def lsb (x: bitvec n) : bool := x.val % 2 = 1
 
-  -- unsigned shift right
-  @[reducible]
-  def ushr (x : bitvec n) (i : ℕ) : bitvec n := ⟨x.val / 2^i,
+  lemma div_pow_mono {x i : ℕ} (h: x < 2^n) : x / 2^i < 2^n :=
     calc
-        x.val / 2^i ≤ x.val : by apply nat.div_le_self
-                ... < 2^n   : by exact x.property⟩
+        x / 2^i ≤ x   : nat.div_le_self x (2^i)
+            ... < 2^n : h
 
-  @[reducible]
+  -- unsigned shift right
+  def ushr (x : bitvec n) (i : ℕ) : bitvec n := ⟨x.val / 2^i, by exact div_pow_mono x.property⟩
+
   def msb (x: bitvec n) : bool := (ushr x (n-1)).val = 1
 
+  lemma sshr_in_range_n_le_i {i x : ℕ} (hx: x < 2^n) (hni: n ≤ i) : 2^n - 2^(n-i) + x/2^i < 2^n :=
+    begin
+      simp [nat.sub_eq_zero_of_le hni],
+      rw div_eq_of_lt,
+      { simp,
+        apply sub_lt_of_pos_le,
+        { dec_trivial_tac },
+        { apply pos_pow_of_pos,
+          dec_trivial_tac,
+        },
+      },
+      { apply nat.lt_of_lt_of_le,
+        { exact hx },
+        { apply pow_le_pow_of_le_right,
+          dec_trivial_tac,
+          exact hni,
+        },
+      },
+    end
+
+  lemma sshr_in_range_i_lt_n_2 {i x : ℕ} (hx: x < 2^n) (hni: i < n) : 2^n - 2^(n-i) + x/2^i < 2^n :=
+    begin
+      cases i, -- This is slightly annoying, but we need to prove
+               -- the i = 0 case separately so we can use i > 0
+               -- for sub_lt_of_pos_le as the argument to
+               -- pow_lt_pow_of_lt_right in the other case.
+      case nat.zero
+      { simp, rw nat.sub_self (2^n), simp, exact hx },
+      case nat.succ
+      { have i_lt_n : succ i ≤ n,
+        { apply le_of_lt hni },
+        have : x/2^succ i < 2^(n-succ i),
+        { apply div_lt_of_lt_mul,
+          apply pos_pow_of_pos,
+          dec_trivial_tac,
+          rw [pow_mul, add_sub_of_le],
+          apply hx,
+          apply i_lt_n
+        },
+        apply sub_add_lt_self (2^n) (2^(n-succ i)) (x/2^(succ i)) _ this,
+        apply pow_lt_pow_of_lt_right (lt_succ_self _)
+                                     (sub_lt_of_pos_le _ _ (nat.zero_lt_succ i) i_lt_n)
+      }
+    end
+
+  lemma sshr_in_range_i_lt_n_i_pos {i x : ℕ} (hx: x < 2^n) (hni: i < n) (hipos: i > 0)
+  : 2^n - 2^(n-i) + x/2^i < 2^n :=
+    begin
+      { have i_le_n : i ≤ n, { apply le_of_lt hni },
+        have x_div_lt : x/2^i < 2^(n-i),
+        { apply div_lt_of_lt_mul,
+          apply pos_pow_of_pos,
+          dec_trivial_tac,
+          rw [pow_mul, add_sub_of_le],
+          apply hx,
+          apply i_le_n
+        },
+        apply sub_add_lt_self (2^n) (2^(n-i)) (x/2^i) _ x_div_lt,
+        apply pow_lt_pow_of_lt_right,
+        { dec_trivial_tac },
+        { apply sub_lt_of_pos_le i n hipos,
+          apply le_of_lt hni
+        },
+      }
+  end
+
+  lemma sshr_in_range_i_lt_n {i x : ℕ} (hx: x < 2^n) (hni: i < n) : 2^n - 2^(n-i) + x/2^i < 2^n :=
+    begin
+      -- We case on i because when i is positive, the cruxt of the
+      -- proof is applying pow_lt_pow_of_lt_right (which requires i > 0)
+      -- (see sshr_in_range_i_lt_n_i_pos).
+      --
+      -- The case when i = 0 basically follows from hx once you
+      -- simplify.
+      by_cases i_cmp_zero : i > 0,
+      { apply sshr_in_range_i_lt_n_i_pos hx hni i_cmp_zero },
+      { have i_zero : i = 0,
+        { apply eq_zero_of_le_zero,
+          apply le_of_not_gt i_cmp_zero,
+        },
+        simp [i_zero, nat.sub_self (2^n)],
+        exact hx
+      },
+    end
+
+  lemma sshr_in_range {i x : ℕ} (h: x < 2^n) : 2^n - 2^(n-i) + x/2^i < 2^n :=
+      begin
+        by_cases this : n ≤ i,
+        { apply sshr_in_range_n_le_i h this },
+        { apply sshr_in_range_i_lt_n h (lt_of_not_ge this) },
+      end
+
   -- signed shift right
-  @[reducible]
   def sshr (x: bitvec n) (i:ℕ) : bitvec n :=
     -- When the sign bit is set in x, (msb x = 1), then we would like
     -- the result of sshr x i, to have the top i bits set.
@@ -162,52 +288,11 @@ section shift
     let sign := if msb x then upper_bits else 0 in
     ⟨ sign + (ushr x i).val,
       begin
-        simp [sign],
-        cases (msb x),
+        simp [sign], cases (msb x),
         case bool.ff
-        { simp [ushr],
-          calc
-            x.val / 2^i ≤ x.val : by apply nat.div_le_self
-                    ... < 2^n   : x.property
-        },
+        { simp [ushr], apply div_pow_mono x.property },
         case bool.tt
-        { simp [upper_bits, sign, ushr],
-          by_cases this : n ≤ i,
-          { rw nat.sub_eq_zero_of_le this,
-            simp,
-            rw div_eq_of_lt,
-            simp,
-            apply sub_lt_of_pos_le,
-            dec_trivial_tac,
-            apply pos_pow_of_pos,
-            dec_trivial_tac,
-            calc
-              x.val < 2^n : x.property
-                ... ≤ 2^i : pow_le_pow_of_le_right (by dec_trivial_tac) this
-          },
-          { cases i, -- This is slightly annoying, but we need to prove
-                     -- the i = 0 case separately so we can use i > 0
-                     -- for sub_lt_of_pos_le as the argument to
-                     -- pow_lt_pow_of_lt_right in the other case.
-            -- case nat.zero
-            { simp, rw nat.sub_self (2^n), simp, exact x.property },
-            -- case nat.succ
-            { have i_lt_n : succ i ≤ n,
-              { apply le_of_not_ge this },
-              have : x.val/2^succ i < 2^(n-succ i),
-              { apply div_lt_of_lt_mul,
-                apply pos_pow_of_pos,
-                dec_trivial_tac,
-                rw [pow_mul, add_sub_of_le],
-                apply x.property,
-                apply i_lt_n
-              },
-              apply sub_add_lt_self (2^n) (2^(n-succ i)) (x.val/2^(succ i)) _ this,
-              apply pow_lt_pow_of_lt_right (lt_succ_self _)
-                                           (sub_lt_of_pos_le _ _ (nat.zero_lt_succ i) i_lt_n)
-            }
-          }
-        }
+        { apply sshr_in_range x.property }
       end⟩
 
 end shift
@@ -248,11 +333,9 @@ section bitwise
     apply bit_lt_pow2 (p _ _),
   end
 
-  @[reducible]
   def bitwise {w:ℕ} (f: bool → bool → bool) (x y : bitvec w) : bitvec w :=
     ⟨fin_bitwise f w x.val y.val, bitwise_lt _ _ _ _⟩
 
-  @[reducible]
   def not {w:ℕ} (x: bitvec w) : bitvec w := ⟨2^w - x.val - 1,
     begin
       have xval_pos : 0 < x.val + 1,
@@ -262,11 +345,8 @@ section bitwise
       apply (succ_pos 1)
     end⟩
 
-  @[reducible]
   def and {w:ℕ} : bitvec w → bitvec w → bitvec w := bitwise band
-  @[reducible]
   def or  {w:ℕ} : bitvec w → bitvec w → bitvec w := bitwise bor
-  @[reducible]
   def xor {w:ℕ} : bitvec w → bitvec w → bitvec w := bitwise bxor
 
 end bitwise
@@ -274,7 +354,6 @@ end bitwise
 section arith
   variable {n : ℕ}
 
-  @[reducible]
   protected def neg (x : bitvec n) : bitvec n :=
     ⟨if x.val = 0 then 0 else 2^n - x.val,
      begin
@@ -289,17 +368,14 @@ section arith
       end⟩
 
   -- Add with carry (no overflow)
-  @[reducible]
   def adc (x y : bitvec n) (c : bool) : bitvec n × bool :=
     let c₁ := if c then 1 else 0,
         r  := x.val + y.val + c₁ in
-    ⟨ ⟨r % 2^n, by simp [in_range] ⟩, r ≥ 2^n ⟩
+    ⟨ ⟨r % 2^n, by simp ⟩, r ≥ 2^n ⟩
 
-  @[reducible]
   protected def add (x y : bitvec n) : bitvec n := (adc x y ff).1
 
   -- Subtract with borrow
-  @[reducible]
   def sbb (x y : bitvec n) (b : bool) : bool × bitvec n :=
     let b₁ : bitvec n := if b then 1 else 0,
         r  := match bitvec.adc x (bitvec.neg y) ff with
@@ -307,16 +383,14 @@ section arith
               end
     in ⟨ if b then y.val + 1 > x.val else y.val > x.val , r.1 ⟩
 
-  @[reducible]
   protected def sub (x y : bitvec n) : bitvec n := (sbb x y ff).2
 
   instance : has_add (bitvec n)  := ⟨bitvec.add⟩
   instance : has_sub (bitvec n)  := ⟨bitvec.sub⟩
   instance : has_neg (bitvec n)  := ⟨bitvec.neg⟩
 
-  @[reducible]
   protected def mul (x y : bitvec n) : bitvec n :=
-    ⟨ (x.val * y.val) % 2^n, by simp [in_range] ⟩
+    ⟨ (x.val * y.val) % 2^n, by simp ⟩
 
   instance : has_mul (bitvec n)  := ⟨bitvec.mul⟩
 end arith
@@ -324,17 +398,12 @@ end arith
 section comparison
   variable {n : ℕ}
 
-  @[reducible]
   def uborrow (x y : bitvec n) : bool := prod.fst (sbb x y ff)
 
-  @[reducible]
   def ult (x y : bitvec n) : Prop := uborrow x y
-  @[reducible]
   def ugt (x y : bitvec n) : Prop := ult y x
 
-  @[reducible]
   def ule (x y : bitvec n) : Prop := ¬ (ult y x)
-  @[reducible]
   def uge (x y : bitvec n) : Prop := ule y x
 
   def sborrow : Π {n : ℕ}, bitvec n → bitvec n → bool
@@ -347,13 +416,9 @@ section comparison
     | (tt, tt) := uborrow (bitvec.neg y) (bitvec.neg x) -- -x < -y when y < x
     end
 
-  @[reducible]
   def slt (x y : bitvec n) : Prop := sborrow x y
-  @[reducible]
   def sgt (x y : bitvec n) : Prop := slt y x
-  @[reducible]
   def sle (x y : bitvec n) : Prop := ¬ (slt y x)
-  @[reducible]
   def sge (x y : bitvec n) : Prop := sle y x
 
 end comparison
@@ -361,15 +426,12 @@ end comparison
 section conversion
   variable {α : Type}
 
-  @[reducible]
-  protected def of_nat (n : ℕ) (x:ℕ) : bitvec n := ⟨ x % 2^n, by simp [in_range] ⟩
+  protected def of_nat (n : ℕ) (x:ℕ) : bitvec n := ⟨ x % 2^n, by simp ⟩
 
-  @[reducible]
   protected def of_int : Π (n : ℕ), int → bitvec (succ n)
   | n (int.of_nat m)          := bitvec.of_nat (succ n) m
   | n (int.neg_succ_of_nat m) := bitvec.neg (bitvec.of_nat (succ n) m)
 
-  @[reducible]
   protected def to_nat {n : nat} (v : bitvec n) : nat := v.val
 
   theorem of_nat_to_nat {n : ℕ} (x : bitvec n)
@@ -400,3 +462,16 @@ end bitvec
 
 instance {n} {x y : bitvec n} : decidable (bitvec.ult x y) := bool.decidable_eq _ _
 instance {n} {x y : bitvec n} : decidable (bitvec.ugt x y) := bool.decidable_eq _ _
+
+def bitvec_pow {n:ℕ} : bitvec n → ℕ → bitvec n
+  | x k := ⟨ (x.val^k) % 2^n, by simp ⟩
+
+instance bitvec_has_pow {n:ℕ} : has_pow (bitvec n) ℕ := ⟨bitvec_pow⟩
+
+instance {n:ℕ} : decidable_eq (bitvec n) := subtype.decidable_eq
+
+/- TODO: it would be good to prove a few properties like this one:
+lemma append_unfold (n m : ℕ) (x : bitvec m) (y: bitvec n)
+  : bitvec.append x y = (bitvec.zext n x) * (2^n : bitvec (m + n)) +
+                        (bitvec.cong (nat.add_comm _ _) (bitvec.zext m y))
+-/
