lean/common.lean
@@ -504,6 +504,7 @@ instance (w:ℕ) : has_neg  (expression (bv w)) := ⟨bvneg⟩
 
 def adc         {w:ℕ} (x : expression (bv w)) (y : expression (bv w)) (b : expression bit) : expression (bv w) := prim.adc   w x y b
 def bswap       {w:ℕ} (v : expression (bv w))                                              : expression (bv w) := prim.bswap w v
+-- TODO: quot should probably be an action to emulate generating an interrupt
 def quot        {w:ℕ} (x : expression (bv w)) (y : expression (bv w))                      : expression (bv w) := prim.quot  w x y
 def rem         {w:ℕ} (x : expression (bv w)) (y : expression (bv w))                      : expression (bv w) := prim.rem   w x y
 def signed_quot {w:ℕ} (x : expression (bv w)) (y : expression (bv w))                      : expression (bv w) := prim.squot w x y
